data/array.lean
@@ -1,0 +1,46 @@
+
+import util.data.fin
+
+universe variables u₀ u₁ u₂
+variables {α : Type u₀} {β β' : Type u₁} {γ : Type u₂}
+
+namespace array
+
+open nat
+
+def push_aux {n : ℕ} (x : α) (ar : fin n → α) : fin (succ n) → α
+  | ⟨0,_⟩ := x
+  | ⟨succ i,P⟩ := ar ⟨i,lt_of_succ_lt_succ P⟩
+
+def push {n : ℕ} (x : α) : array α n → array α (succ n)
+  | ⟨ ar ⟩ := ⟨ push_aux x ar ⟩
+
+def pop {n : ℕ} : array α (succ n) → array α n
+  | ⟨ ar ⟩ := ⟨ ar ∘ fin.next ⟩
+
+def head {n : ℕ} : array α (succ n) → α
+  | ⟨ ar ⟩ := ar 0
+
+lemma push_head_pop {n : ℕ} (xs : array α (succ n))
+: push (head xs) (pop xs) = xs := sorry
+
+lemma rev_iterate_push {n : ℕ}
+  (x : α) (xs : array α n)
+  (i : β)
+  (f : fin (succ n) → α → β → β)
+: rev_iterate (push x xs) i f = f 0 x (rev_iterate xs i (f ∘ fin.next)) :=
+begin
+  revert x xs,
+  induction n with n IH ; intros x xs,
+  { cases xs with xs,
+    unfold push push_aux rev_iterate rev_iterate_aux,
+    simp,
+    unfold read data push_aux,
+    rw fin.zero_def' },
+  { rw [-push_head_pop xs,IH],
+    unfold function.comp,
+    rw push_head_pop xs,
+    admit }
+end
+
+end array
